Port incremental lemmas about Blake2

specs/lemmas/Spec.Blake2.Incremental.fst
@@ -11,11 +11,21 @@ open FStar.Mul
 
 friend Spec.Agile.Hash
 
-let blake2_is_hash_incremental a input =
-  admit()
+#push-options "--fuel 0 --ifuel 0 --z3rlimit 200"
+// let blake2_is_hash_incremental a input =
+//   let blocks, last = Lib.UpdateMulti.split_at_last_lazy (block_length a) input in
+//   let s = init a in
 
-(* This proof works, but occasionally sends F* on an infinite loop.
-   Commenting out for now
+//   let a = to_blake_alg a in
+//   let n_blocks, l_last = Spec.Blake2.split a (S.length input) in
+//   let s1 = Lib.LoopCombinators.repeati n_blocks (Spec.Blake2.blake2_update1 a 0 input) s in
+//   let s2 = Lib.LoopCombinators.repeati n_blocks (Spec.Blake2.blake2_update1 a 0 blocks) s in
+//   Lib.Sequence.Lemmas.repeati_extensionality n_blocks (Spec.Blake2.blake2_update1 a 0 input)
+//     (Spec.Blake2.blake2_update1 a 0 blocks) s;
+//   S.lemma_eq_intro (S.slice input (S.length input - l_last) (S.length input)) last;
+//   S.lemma_eq_intro (S.slice last (S.length last - l_last) (S.length last)) last
+
+
 /// AF: While this proof should be conceptually simple, and very similar to the proof in Hacl.Streaming.Blake2,
 /// F* struggles heavily with the dependent pairs for the state and slighty type mismatches...
 /// In particular, even proving that update_multi is equal to its definition can be challenging.
@@ -27,21 +37,20 @@ let update1_ext
   (a:blake_alg)
   (input:bytes{S.length input `less_than_max_input_length` a})
   (bs:bytes{bs == fst (split_blocks a input)})
-  (i:nat{i < S.length bs / block_length a}) (acc:words_state' a)
+  (i:nat{i < S.length bs / block_length a}) (acc:words_state a)
   : Lemma
      ( Spec.Blake2.blake2_update1 (to_blake_alg a) 0 input i acc == Spec.Blake2.blake2_update1 (to_blake_alg a) 0 bs i acc)
   = assert (Spec.Blake2.get_blocki (to_blake_alg a) input i `S.equal` Spec.Blake2.get_blocki (to_blake_alg a) bs i)
 
 val blake2b_update_incremental
   (input : bytes {S.length input `less_than_max_input_length` Blake2B})
-  (s: words_state' Blake2B & nat)
+  (s: words_state Blake2B)
   : Lemma
-    (requires snd s == 0)
     (ensures
-      S.equal (Spec.Blake2.blake2_update (to_blake_alg Blake2B) 0 S.empty input (fst s))
+      S.equal (Spec.Blake2.blake2_update (to_blake_alg Blake2B) 0 S.empty input s)
               (let bs, l = split_blocks Blake2B input in
-                let s:words_state' Blake2B & nat = update_multi Blake2B s bs in
-                update_last Blake2B (fst s) (S.length bs) l))
+                let s:words_state Blake2B = update_multi Blake2B s 0 bs in
+                update_last Blake2B s (S.length bs) l))
 
 /// Unclear why this proof needs to be spelled out more than the one for blake2s
 let blake2b_update_incremental input s =
@@ -49,15 +58,15 @@ let blake2b_update_incremental input s =
   let a' = to_blake_alg Blake2B in
 
   let bs, l = split_blocks a input in
-  let s_m:words_state' a & nat = update_multi a s bs in
+  let s_m:words_state a = update_multi a s 0 bs in
 
 
   let nb = S.length bs / block_length a in
 
-  let s_m_def = Lib.LoopCombinators.repeati nb (Spec.Blake2.blake2_update1 a' 0 bs) (fst s) in
-  assert (fst s_m == s_m_def);
+  let s_m_def = Lib.LoopCombinators.repeati nb (Spec.Blake2.blake2_update1 a' 0 bs) s in
+  assert (s_m == s_m_def);
 
-  Spec.Blake2.Alternative.lemma_spec_equivalence_update a' 0 S.empty input (fst s);
+  Spec.Blake2.Alternative.lemma_spec_equivalence_update a' 0 S.empty input s;
 
   assert ((S.empty `S.append` input) `S.equal` input);
   let nb', rem = Spec.Blake2.split a' (S.length input) in
@@ -65,38 +74,36 @@ let blake2b_update_incremental input s =
 
   FStar.Math.Lemmas.cancel_mul_div (S.length bs) (block_length a);
   assert (nb == nb');
-  let s_m' = Lib.LoopCombinators.repeati nb' (Spec.Blake2.blake2_update1 a' 0 input) (fst s) in
+  let s_m' = Lib.LoopCombinators.repeati nb' (Spec.Blake2.blake2_update1 a' 0 input) s in
 
-  let aux () : Lemma (s_m' == Lib.LoopCombinators.repeati nb' (Spec.Blake2.blake2_update1 a' 0 bs) (fst s))  =
+  let aux () : Lemma (s_m' == Lib.LoopCombinators.repeati nb' (Spec.Blake2.blake2_update1 a' 0 bs) s)  =
     Classical.forall_intro_2 (update1_ext a input bs);
     Lib.Sequence.Lemmas.repeati_extensionality nb' (Spec.Blake2.blake2_update1 a' 0 input)
-      (Spec.Blake2.blake2_update1 a' 0 bs) (fst s)
+      (Spec.Blake2.blake2_update1 a' 0 bs) s
   in
   aux ();
-  assert (s_m' == fst s_m)
+  assert (s_m' == s_m)
 
 val blake2s_update_incremental
   (input : bytes {S.length input `less_than_max_input_length` Blake2S})
-  (s: words_state' Blake2S & nat)
+  (s: words_state Blake2S)
   : Lemma
-    (requires snd s == 0)
     (ensures
-      S.equal (Spec.Blake2.blake2_update (to_blake_alg Blake2S) 0 S.empty input (fst s))
+      S.equal (Spec.Blake2.blake2_update (to_blake_alg Blake2S) 0 S.empty input s)
               (let bs, l = split_blocks Blake2S input in
-                let s:words_state' Blake2S & nat = update_multi Blake2S s bs in
-                update_last Blake2S (fst s) (S.length bs) l))
-
+                let s:words_state Blake2S = update_multi Blake2S s 0 bs in
+                update_last Blake2S s (S.length bs) l))
 
 let blake2s_update_incremental input s =
   let a = Blake2S in
   let a' = to_blake_alg Blake2S in
 
   let bs, l = split_blocks a input in
-  let s_m:words_state' a & nat = update_multi a s bs in
+  let s_m:words_state a = update_multi a s 0 bs in
 
   let nb = S.length bs / block_length a in
 
-  Spec.Blake2.Alternative.lemma_spec_equivalence_update a' 0 S.empty input (fst s);
+  Spec.Blake2.Alternative.lemma_spec_equivalence_update a' 0 S.empty input s;
   assert ((S.empty `S.append` input) `S.equal` input);
 
   let nb', rem = Spec.Blake2.split a' (S.length input) in
@@ -104,23 +111,22 @@ let blake2s_update_incremental input s =
   FStar.Math.Lemmas.cancel_mul_div (S.length bs) (block_length a);
   assert (nb == nb');
 
-  let s_m' = Lib.LoopCombinators.repeati nb' (Spec.Blake2.blake2_update1 a' 0 input) (fst s) in
+  let s_m' = Lib.LoopCombinators.repeati nb' (Spec.Blake2.blake2_update1 a' 0 input) s in
 
   Lib.Sequence.Lemmas.repeati_extensionality nb (Spec.Blake2.blake2_update1 a' 0 input)
-     (Spec.Blake2.blake2_update1 a' 0 bs) (fst s);
-  assert (s_m' == fst s_m)
+     (Spec.Blake2.blake2_update1 a' 0 bs) s;
+  assert (s_m' == s_m)
 
 val blake2_update_incremental
   (a:blake_alg)
   (input : bytes {S.length input `less_than_max_input_length` a})
-  (s: words_state' a & nat)
+  (s: words_state a)
   : Lemma
-    (requires snd s == 0)
     (ensures
-      S.equal (Spec.Blake2.blake2_update (to_blake_alg a) 0 S.empty input (fst s))
+      S.equal (Spec.Blake2.blake2_update (to_blake_alg a) 0 S.empty input s)
               (let bs, l = split_blocks a input in
-                let s:words_state' a & nat = update_multi a s bs in
-                update_last a (fst s) (S.length bs) l))
+                let s:words_state a = update_multi a s 0 bs in
+                update_last a s (S.length bs) l))
 
 let blake2_update_incremental a input s = match a with
   | Blake2B -> blake2b_update_incremental input s
@@ -131,8 +137,7 @@ let blake2_is_hash_incremental a input =
   let n_blocks, l_last = Spec.Blake2.split a' (S.length input) in
   let blocks, last = Lib.UpdateMulti.split_at_last_lazy (block_length a) input in
   let s_i = Spec.Blake2.blake2_init_hash a' 0 (Spec.Blake2.max_output (to_blake_alg a)) in
-  let s_i': words_state' a & nat = init a in
-  assert (s_i == fst s_i');
+  let s_i': words_state a = init a in
+  assert (s_i == s_i');
 
   blake2_update_incremental a input s_i'
-*)
